u(x,t) = \sum_{n=1}^{\infty} B_n \sin\left(\frac{n\pi x}{L}\right) e^{-\alpha \left(\frac{n\pi}{L}\right)^2 t}, \quad \text{where } B_n = \frac{2}{L} \int_0^L f(x) \sin\left(\frac{n\pi x}{L}\right) dx, \quad f(x) = u(x,0)
u(x,t) = \frac{1}{2} \left[f(x+ct) + f(x-ct)\right] + \frac{1}{2c} \int_{x-ct}^{x+ct} g(s)\, ds, \quad \text{with } u(x,0) = f(x), \quad u_t(x,0) = g(x)
\mathcal{L}\{y''(t)\} = s^2 Y(s) - s y(0) - y'(0), \quad \text{so } \mathcal{L}\{y'' + 4y' + 4y\} = \mathcal{L}\{f(t)\} \Rightarrow (s^2 + 4s + 4)Y(s) - s y(0) - y'(0) = F(s)
f(x) = \frac{a_0}{2} + \sum_{n=1}^{\infty} \left[a_n \cos\left(\frac{n\pi x}{L}\right) + b_n \sin\left(\frac{n\pi x}{L}\right)\right], \quad \text{where } a_n = \frac{1}{L} \int_{-L}^{L} f(x) \cos\left(\frac{n\pi x}{L}\right)\, dx, \quad b_n = \frac{1}{L} \int_{-L}^{L} f(x) \sin\left(\frac{n\pi x}{L}\right)\, dx
u(x,y) = \sum_{n=1}^{\infty} \left(A_n \sinh\left(\frac{n\pi y}{a}\right) + B_n \cosh\left(\frac{n\pi y}{a}\right)\right) \sin\left(\frac{n\pi x}{a}\right), \quad \text{with } A_n = \frac{2}{a \sinh\left(\frac{n\pi b}{a}\right)} \int_0^a f(x) \sin\left(\frac{n\pi x}{a}\right) dx
